todo.md
@@ -5,15 +5,15 @@
     - [ ] tactic for monotonicity in predicate calculus
     - [x] reduce soundness of leads-to properties to assumptions about transient
     - [x] prove soundness of unitb.models.sched
-    - [ ] prove that unitb.models.sched are inhabited
+    - [x] prove that unitb.models.sched are inhabited
     - [x] in unitb.models.sched, give a rule that relies only on predicate
       calculus and UNITY logic
     - [ ] study model where the invariant is encoded in the state space
-    - [ ] generalize transient_rule (from unity.models.nondet) and put in
+    - [ ] ~~generalize transient_rule (from unity.models.nondet) and put in
       type class so that it becomes a requirement that other models
-      can subscribe to
+      can subscribe to~~
     - [ ] models
-      - [ ] in nondet, push the reference to liveness out of transient
+      - [x] in nondet, push the reference to liveness out of transient
     - [ ] refinement
       - [x] schedules
       - [x] simulation
